fairness/lawyer/obligations_em.v
@@ -1,0 +1,115 @@
+From iris.proofmode Require Import tactics.
+From iris.algebra Require Import auth gmap gset excl gmultiset big_op mono_nat.
+From trillium.fairness Require Import fairness locales_helpers execution_model.
+From trillium.fairness.lawyer Require Import obligations_model obls_utils obligations_resources. 
+
+
+
+Section ObligationsEM.
+
+  Context {DegO LevelO: ofe}.
+  Context `{OfeDiscrete DegO} `{OfeDiscrete LevelO}
+    `{@LeibnizEquiv (ofe_car LevelO) (ofe_equiv LevelO)}
+  .
+
+  Let Degree := ofe_car DegO.
+  Let Level := ofe_car LevelO.
+
+  (* Context {Locale: Type}. *)
+  Context {Λ: language}.
+  Context `{Countable (locale Λ)}.
+  Let Locale := locale Λ.
+
+  Context {LIM_STEPS: nat}.
+  Context (OP: ObligationsParams Degree Level Locale LIM_STEPS).
+  Let OM := ObligationsModel OP.
+
+  Definition threads_own_obls (c: cfg Λ) (δ: mstate OM) :=
+    locales_of_cfg c = dom $ ps_obls OP δ. 
+    
+  Lemma locale_nofork_step_obls_pres c1 c2 τ θ δ1 δ2
+    (STEP: locale_step c1 (Some τ) c2)
+    (TH_OWN: threads_own_obls c1 δ1)
+    (TRANS: progress_step OP δ1 θ δ2)
+    (NOFORK: locales_of_cfg c2 = locales_of_cfg c1)
+    :
+    threads_own_obls c2 δ2.
+  Proof.
+    destruct c1 as [tp1 σ1], c2 as [tp2 σ2].
+    red. rewrite NOFORK.
+    eapply progress_step_obls_pres in TRANS; [| apply obls_eq_init].
+    rewrite TRANS. done. 
+  Qed.
+      
+  Definition obls_valid_evolution_step
+    (σ1: cfg Λ) (oζ: olocale Λ) (σ2: cfg Λ)
+    (δ1: mstate OM) (ℓ: mlabel OM) (δ2: mstate OM) :=
+      mtrans δ1 ℓ δ2 /\
+      oζ = Some ℓ                
+  .
+
+  Definition obls_si `{!ObligationsGS OP Σ}
+    (σ: cfg Λ) (δ: mstate OM): iProp Σ :=
+      obls_msi _ δ ∗
+      ⌜ threads_own_obls σ δ ⌝ ∗
+      ⌜ dom_phases_obls OP δ ⌝
+  . 
+
+  Definition obls_init_resource `{!ObligationsGS OP Σ}
+    (δ: mstate OM) (_: unit): iProp Σ :=
+    own (obls_cps _) (◯ (cps_repr _ $ ps_cps _ δ)) ∗
+    own (obls_sigs _) (◯ (sig_map_repr $ ps_sigs _ δ)) ∗
+    own (obls_obls _) (◯ (obls_map_repr $ ps_obls _ δ)) ∗
+    own (obls_eps _) (◯ (eps_repr _ $ ps_eps _ δ)) ∗
+    own (obls_phs _) (◯ (phases_repr $ ps_phases _ δ)) ∗
+    own (obls_exc_lb _) (◯MN (ps_exc_bound _ δ))
+  .
+
+  Definition obls_is_init_st (σ: cfg Λ) (δ: mstate OM) :=
+    exists τ0,
+      let R := {[ τ0 ]} in
+      locales_of_cfg σ = R /\ dom $ ps_obls OP δ = R /\ dom $ ps_phases OP δ = R. 
+
+  Program Definition ObligationsEM: ExecutionModel Λ OM :=
+    {| 
+      em_preGS := ObligationsPreGS OP;
+      em_GS := ObligationsGS OP;
+      em_Σ := obls_Σ OP;
+      em_valid_evolution_step := obls_valid_evolution_step;
+      em_thread_post Σ `{!ObligationsGS OP Σ} :=
+        fun τ => (obls _ τ ∅)%I;
+      em_msi Σ `{!ObligationsGS OP Σ} := obls_si;
+      em_init_param := unit; (* ? *)
+      em_init_resource (Σ: gFunctors) `{!ObligationsGS OP Σ} := obls_init_resource;
+      em_is_init_st := obls_is_init_st;
+    |}.
+  Next Obligation.
+    simpl. intros ? PRE δ σ ? INIT. iStartProof.
+    iMod (own_alloc (● (cps_repr _ $ ps_cps _  δ) ⋅ ◯ _)) as (?) "[CPa CPf]".
+    { by apply auth_both_valid_2. }
+    iMod (own_alloc (● (sig_map_repr (ps_sigs _ δ)) ⋅ ◯ _)) as (?) "[SIGSa SIGSf]".
+    { apply auth_both_valid_2; [| reflexivity].
+      rewrite /sig_map_repr.
+      intros s. destruct lookup eqn:L; [| done].
+      apply lookup_fmap_Some in L. 
+      destruct L as ([l b]&<-&?).
+      done. }
+    iMod (own_alloc (● (obls_map_repr $ ps_obls _ δ) ⋅ ◯ _)) as (?) "[OBLSa OBLSf]". 
+    { apply auth_both_valid_discrete. split; [reflexivity| ].
+      intros τ. rewrite lookup_fmap. 
+      by destruct lookup. }
+    iMod (own_alloc (● (eps_repr _ $ ps_eps _ δ) ⋅ ◯ _)) as (?) "[EPSa EPSf]". 
+    { by apply auth_both_valid_2. }
+    iMod (own_alloc (● (phases_repr $ ps_phases _ δ) ⋅ ◯ _)) as (?) "[PHa PHf]". 
+    { apply auth_both_valid_2; [| reflexivity].
+      rewrite /phases_repr. intros τ. destruct lookup eqn:L; [| done].
+      rewrite lookup_fmap_Some in L. destruct L as (? & <- & L). done. }
+    iMod (own_alloc (●MN (ps_exc_bound _ δ) ⋅ mono_nat_lb _)) as (?) "[LBa LBf]".
+    { apply mono_nat_both_valid. reflexivity. }
+    iModIntro. iExists {| obls_pre := PRE; |}.
+    iFrame.
+    iPureIntro. 
+    red in INIT. destruct INIT as (?&?&?&?). set_solver.  
+  Qed.
+
+End ObligationsEM.
